Tests/DTLC/Sanity.lean
@@ -81,12 +81,37 @@ def apply1stOn2ndFnOnTuple : TrmClosed :=
     (.depApply apply1stOn2ndFn identityFn)
     false
 
+def applyIdentityFnOnItself : TrmClosed :=
+  .depApply Trm.identityFn Trm.identityFn
+
+def identityFnOnFalse2 : TrmClosed :=
+  .depApply applyIdentityFnOnItself false
+
 end Trm
 
 namespace Runtime
 
 
 end Runtime
+
+namespace Eval
+
+example : Definitional.eval Trm.false 0 = none := rfl
+example : Definitional.eval Trm.false 1 = some ((Val.primitive "false") : Val SemCarrier) := rfl
+example : Definitional.eval Trm.false 2 = some ((Val.primitive "false") : Val SemCarrier) := rfl
+example : Definitional.eval Trm.identityFnOnFalse 0 = none := rfl
+example : Definitional.eval Trm.identityFnOnFalse 1 = some ((Val.primitive "false") : Val SemCarrier) := rfl
+example : Definitional.eval Trm.get1stOnTuple 1 = none := rfl
+example : Definitional.eval Trm.get1stOnTuple 2 = some ((Val.primitive "false") : Val SemCarrier) := rfl
+example : Definitional.eval Trm.get2ndOnTuple 2 = some ((Val.primitive "true") : Val SemCarrier) := rfl
+example : Definitional.eval Trm.apply1stOn2ndFnOnTuple 2 = none := rfl
+example : Definitional.eval Trm.apply1stOn2ndFnOnTuple 3 = some ((Val.primitive "false") : Val SemCarrier) := rfl
+example : (Definitional.eval Trm.applyIdentityFnOnItself 0).isNone = true := rfl
+example : (Definitional.eval Trm.applyIdentityFnOnItself 1).isSome = true := rfl
+example : Definitional.eval Trm.identityFnOnFalse2 1 = none := rfl
+example : Definitional.eval Trm.identityFnOnFalse2 2 = some ((Val.primitive "false") : Val SemCarrier) := rfl
+
+end Eval
 
 -- namespace Eval
 
