Lp2lc/Active/DTLC/AGENTS.md
@@ -8,7 +8,8 @@ This directory contain syntax, typing/semantic/evaluation rules and proof of sou
 - absolute type safety, unsafe/noncomputable/partial definition is NOT allowed.
 - All definition must be with a short docString explaining their necessity.
 - All function/constructor arguments must be named.
-- prefer dot-notation for invoking multi-parameter functions and inductive destructors.
+- Multiple cases in pattern matching should never be in 1 line, each line should start with `|`.
+- Prefer dot-notation for invoking multi-parameter functions and inductive destructors.
 - Do NOT repeat yourself, break repeated condition in pattern matching into multiple layers of pattern matchings if applicable.
 - Avoid leaky abstraction: top-level public APIs should only contain interpreter/compiler API (e.g. type-checking, evaluation). evaluator/checker helpers of PHOAS should be kept local to to each API, only helpers reused by multiple public APIs may be private.
 - Avoid generic universe, use static Prop/Type/Sort level on-demand (Type, Type 1, Type 2)
